[[S4.pdf]]

1. Demuestre usando la definición formal:

- $\lim_{x \to 0} \frac{x}{1 + \sin (x^{2})} = 0$.

Sea $\varepsilon > 0$, escogeremos $\delta = \varepsilon$ y asumiremos que $0 < |x| < \delta$. Entonces:

$$
\left|\frac{x}{1 + \sin^{2}(x)}\right| = \frac{|x|}{1 + \sin^{2}(x)}
$$

Pero

$$
\begin{gather}
0 \leq \sin^{2}(x) \leq 1 \\
1 \leq 1 + \sin^{2}(x) \leq 2 \\
\frac{1}{2} \leq \frac{1}{1 + \sin^{2}(x)} \leq 1
\end{gather}
$$

Así que

$$
\begin{align}
\frac{|x|}{1 + \sin^{2}(x)} < |x| < \delta = \varepsilon
\end{align}
$$
$$\qed$$
4. Calcule $\lim_{x \to 0} \frac{\cos^{3}(x) - \cos^{2} - \cos(x) + 1}{\tan^{2}(x) - \sin^{2}(x)}$

$$
\begin{align}
\lim_{x \to 0} \frac{\cos^{3}(x) - \cos^{2} - \cos(x) + 1}{\tan^{2}(x) - \sin^{2}(x)} &= \lim_{x \to 0} \frac{(1 - \cos^{2}(x)) - \cos(x)(1 - \cos^{2}(x))}{\tan^{2} - \sin^{2}(x)} \\
&= \lim_{x \to 0} \frac{\sin^{2}(x) - \sin^{2}\cos(x)}{\tan^{2} - \sin^{2}(x)} \\
&= \lim_{x \to 0} \frac{\cancel{\sin^{2}(x)}(1 - \cos(x))}{\cancel{\sin^{2}(x)}(\sec^{2}(x) - 1)} \\
&= \lim_{x \to 0}  \frac{1 - \cos(x)}{\tan^{2}(x)} \\
&= \lim_{x \to 0} \frac{\cos^{2}(x)(1 - \cos(x))}{\sin^{2}(x)} \cdot \frac{1 + \cos(x)}{1 + \cos(x)} \\
&= \lim_{x \to 0} \frac{\cos^{2}(x)\cancel{\sin^{2}(x)}}{\cancel{\sin^{2}(x)}(1 + \cos(x))} \\
\lim_{x \to 0} \frac{\cos^{3}(x) - \cos^{2} - \cos(x) + 1}{\tan^{2}(x) - \sin^{2}(x)} &= \frac{\cos^{2}(0)}{1 + \cos(0)} = \frac{1}{2}
\end{align}
$$
